Refacorings

indexed_vlsm.v
@@ -10,20 +10,20 @@ Composition of indexed VLSMs.
 Assumes classical logic (excluded middle) and the axiom of choice.
 *)
 
-Definition icomposed_state
+Definition indexed_state
   {index : Set} {message : Type}
   (IS : index -> VLSM message)
   : Type
   :=
   forall i : index, (@state _ (IS i)).
 
-Definition icomposed_label
+Definition indexed_label
   {index : Set} {message : Type}
   (IS : index -> VLSM message)
   : Type
   := sigT (fun i => @label _ (IS i)).
 
-Definition icomposed_proto_message_prop
+Definition indexed_proto_message_prop
   {index : Set} {message : Type}
   (IS : index -> VLSM message)
   (m : message)
@@ -31,39 +31,39 @@ Definition icomposed_proto_message_prop
   :=
   exists i : index, @proto_message_prop message (IS i) m.
 
-Lemma icomposed_proto_message_decidable
+Lemma indexed_proto_message_decidable
   {index : Set} {message : Type}
   (IS : index -> VLSM message)
-  : forall m : message, {icomposed_proto_message_prop IS m} + {~icomposed_proto_message_prop IS m}.
+  : forall m : message, {indexed_proto_message_prop IS m} + {~indexed_proto_message_prop IS m}.
 Proof.
   intros.
   apply excluded_middle_informative.
 Qed.
 
-Definition icomposed_proto_message
+Definition indexed_proto_message
   {index : Set} {message : Type}
   (IS : index -> VLSM message)
-  := { m : message | icomposed_proto_message_prop IS m }.
+  := { m : message | indexed_proto_message_prop IS m }.
 
-Definition icomposed_initial_state_prop
+Definition indexed_initial_state_prop
   {index : Set} {message : Type}
   (IS : index -> VLSM message)
-  (s : icomposed_state IS)
+  (s : indexed_state IS)
   : Prop
   :=
   forall i : index, @initial_state_prop _ (IS i) (s i).
 
-Definition icomposed_initial_state
+Definition indexed_initial_state
   {index : Set} {message : Type}
   (IS : index -> VLSM message)
-  := { s : icomposed_state IS | icomposed_initial_state_prop IS s }.
+  := { s : indexed_state IS | indexed_initial_state_prop IS s }.
 
-Lemma icomposed_protocol_state_inhabited
+Lemma indexed_protocol_state_inhabited
   {index : Set} {message : Type}
   (IS : index -> VLSM message)
-  : inhabited (icomposed_initial_state IS).
+  : inhabited (indexed_initial_state IS).
 Proof.
-  unfold icomposed_initial_state. unfold icomposed_state. unfold icomposed_initial_state_prop.
+  unfold indexed_initial_state. unfold indexed_state. unfold indexed_initial_state_prop.
   assert (Hchoice : exists s : forall i : index, @state _ (IS i), forall i : index, @initial_state_prop _ (IS i) (s i)).
   { apply (non_dep_dep_functional_choice choice). simpl.
     intros i. destruct (@protocol_state_inhabited _ (IS i)) as [[s His]].
@@ -73,34 +73,34 @@ Proof.
   constructor. exists s. assumption.
 Qed.
 
-Definition icomposed_initial_message_prop
+Definition indexed_initial_message_prop
   {index : Set} {message : Type}
   (IS : index -> VLSM message)
-  (m : icomposed_proto_message IS)
+  (m : indexed_proto_message IS)
   : Prop
   :=
   exists (i : index) (mi : @initial_message _ (IS i)), proj1_sig (proj1_sig mi) = proj1_sig m.
 
 
-Lemma icomposed_message_inhabited
+Lemma indexed_message_inhabited
   {index : Set} {message : Type}
   (IS : index -> VLSM message)
   (Hi : inhabited index)
-  : inhabited (icomposed_proto_message IS)
+  : inhabited (indexed_proto_message IS)
   .
 Proof.
-  unfold icomposed_proto_message. unfold icomposed_proto_message_prop.
+  unfold indexed_proto_message. unfold indexed_proto_message_prop.
   destruct Hi as [i]. destruct (@message_inhabited _ (IS i)) as [[m Hpm]].
   constructor. exists m. exists i. assumption.
 Qed.
 
-Lemma icomposed_label_inhabited
+Lemma indexed_label_inhabited
   {index : Set} {message : Type}
   (IS : index -> VLSM message)
   (Hi : inhabited index)
-  : inhabited (icomposed_label IS).
+  : inhabited (indexed_label IS).
 Proof.
-  unfold icomposed_label.
+  unfold indexed_label.
   destruct Hi as [i].
   destruct (@label_inhabited message (IS i)) as [l].
   constructor.
@@ -112,7 +112,7 @@ Definition lift_proto_messageI
   (IS : index -> VLSM message)
   (i : index)
   (mi : @proto_message _ (IS i))
-  : icomposed_proto_message IS.
+  : indexed_proto_message IS.
 destruct mi as [m Hm].
 exists m. exists i. assumption.
 Defined.
@@ -120,12 +120,12 @@ Defined.
 Class EqDec X :=
   eq_dec : forall x y : X, {x = y} + {x <> y}.
 
-Definition icomposed_transition
+Definition indexed_transition
   {index : Set} {message : Type} `{Heqd : EqDec index}
   (IS : index -> VLSM message)
-  (l : icomposed_label IS)
-  (som : icomposed_state IS * option (icomposed_proto_message IS))
-  : icomposed_state IS * option (icomposed_proto_message IS).
+  (l : indexed_label IS)
+  (som : indexed_state IS * option (indexed_proto_message IS))
+  : indexed_state IS * option (indexed_proto_message IS).
 destruct som as [s om].
 destruct l as [i li].
 destruct om as [[m _]|].
@@ -147,11 +147,11 @@ destruct om as [[m _]|].
     * exact (option_map (lift_proto_messageI IS i) om').
 Defined.
 
-Definition icomposed_valid
+Definition indexed_valid
   {index : Set} {message : Type} `{Heqd : EqDec index}
   (IS : index -> VLSM message)
-  (l : icomposed_label IS)
-  (som : icomposed_state IS * option (icomposed_proto_message IS))
+  (l : indexed_label IS)
+  (som : indexed_state IS * option (indexed_proto_message IS))
   : Prop.
 destruct som as [s om].
 destruct l as [i li].
@@ -163,11 +163,11 @@ destruct om as [[m _]|].
 Defined.
 
 
-Definition icomposed_valid_decidable
+Definition indexed_valid_decidable
   {index : Set} {message : Type} `{Heqd : EqDec index}
   (IS : index -> VLSM message)
-  : forall (l : icomposed_label IS) (som : icomposed_state IS * option (icomposed_proto_message IS)),
-  {icomposed_valid IS l som} + {~icomposed_valid IS l som}.
+  : forall (l : indexed_label IS) (som : indexed_state IS * option (indexed_proto_message IS)),
+  {indexed_valid IS l som} + {~indexed_valid IS l som}.
 Proof.
   destruct som as [s om].
   destruct l as [i li]; simpl.
@@ -179,28 +179,28 @@ Proof.
 Qed.
 
 
-Definition icomposed_valid_constrained
+Definition indexed_valid_constrained
   {index : Set} {message : Type} `{Heqd : EqDec index}
   (IS : index -> VLSM message)
-  (constraint : icomposed_label IS -> icomposed_state IS * option (icomposed_proto_message IS) -> Prop)
-  (l : icomposed_label IS)
-  (som : icomposed_state IS * option (icomposed_proto_message IS))
+  (constraint : indexed_label IS -> indexed_state IS * option (indexed_proto_message IS) -> Prop)
+  (l : indexed_label IS)
+  (som : indexed_state IS * option (indexed_proto_message IS))
   :=
-  icomposed_valid IS l som /\ constraint l som.
+  indexed_valid IS l som /\ constraint l som.
 
 
-Definition icomposed_valid_constrained_decidable
+Definition indexed_valid_constrained_decidable
   {index : Set} {message : Type} `{Heqd : EqDec index}
   (IS : index -> VLSM message)
-  {constraint : icomposed_label IS -> icomposed_state IS * option (icomposed_proto_message IS) -> Prop}
-  (constraint_decidable : forall (l : icomposed_label IS) (som : icomposed_state IS * option (icomposed_proto_message IS)), {constraint l som} + {~constraint l som})
-  : forall (l : icomposed_label IS) (som : icomposed_state IS * option (icomposed_proto_message IS)),
-  {icomposed_valid_constrained IS constraint l som} + {~icomposed_valid_constrained IS constraint l som}.
+  {constraint : indexed_label IS -> indexed_state IS * option (indexed_proto_message IS) -> Prop}
+  (constraint_decidable : forall (l : indexed_label IS) (som : indexed_state IS * option (indexed_proto_message IS)), {constraint l som} + {~constraint l som})
+  : forall (l : indexed_label IS) (som : indexed_state IS * option (indexed_proto_message IS)),
+  {indexed_valid_constrained IS constraint l som} + {~indexed_valid_constrained IS constraint l som}.
 Proof.
   intros.
-  unfold icomposed_valid_constrained.
+  unfold indexed_valid_constrained.
   destruct (constraint_decidable l som) as [Hc | Hnc].
-  - destruct (icomposed_valid_decidable IS l som) as [Hv | Hnv].
+  - destruct (indexed_valid_decidable IS l som) as [Hv | Hnv].
     + left. split; try assumption.
     + right. intros [Hv _]. contradiction.
   - right. intros [_ Hc]. contradiction.
@@ -208,149 +208,47 @@ Qed.
 
 (* Free VLSM composition *)
 
-Definition composed_vlsm
+Definition indexed_vlsm
   {index : Set} {message : Type} `{Heqd : EqDec index}
   (IS : index -> VLSM message)
   (Hi : inhabited index)
   : VLSM message
   :=
-  {| state := icomposed_state IS
-  ; label := icomposed_label IS
-  ; proto_message_prop := icomposed_proto_message_prop IS
-  ; proto_message_decidable := icomposed_proto_message_decidable IS
-  ; initial_state_prop := icomposed_initial_state_prop IS
-  ; protocol_state_inhabited := icomposed_protocol_state_inhabited IS
-  ; initial_message_prop := icomposed_initial_message_prop IS
-  ; message_inhabited := icomposed_message_inhabited IS Hi
-  ; label_inhabited := icomposed_label_inhabited IS Hi
-  ; transition := icomposed_transition IS
-  ; valid := icomposed_valid IS
-  ; valid_decidable := icomposed_valid_decidable IS
+  {| state := indexed_state IS
+  ; label := indexed_label IS
+  ; proto_message_prop := indexed_proto_message_prop IS
+  ; proto_message_decidable := indexed_proto_message_decidable IS
+  ; initial_state_prop := indexed_initial_state_prop IS
+  ; protocol_state_inhabited := indexed_protocol_state_inhabited IS
+  ; initial_message_prop := indexed_initial_message_prop IS
+  ; message_inhabited := indexed_message_inhabited IS Hi
+  ; label_inhabited := indexed_label_inhabited IS Hi
+  ; transition := indexed_transition IS
+  ; valid := indexed_valid IS
+  ; valid_decidable := indexed_valid_decidable IS
   |}.
 
 
 (* Constrained VLSM composition *)
 
-Definition composed_vlsm_constrained
+Definition indexed_vlsm_constrained
   {index : Set} {message : Type} `{Heqd : EqDec index}
   (IS : index -> VLSM message)
   (Hi : inhabited index)
-  (constraint : icomposed_label IS -> icomposed_state IS * option (icomposed_proto_message IS) -> Prop)
-  (constraint_decidable : forall (l : icomposed_label IS) (som : icomposed_state IS * option (icomposed_proto_message IS)), {constraint l som} + {~constraint l som})
+  (constraint : indexed_label IS -> indexed_state IS * option (indexed_proto_message IS) -> Prop)
+  (constraint_decidable : forall (l : indexed_label IS) (som : indexed_state IS * option (indexed_proto_message IS)), {constraint l som} + {~constraint l som})
   : VLSM message
   :=
-  {| state := icomposed_state IS
-  ; label := icomposed_label IS
-  ; proto_message_prop := icomposed_proto_message_prop IS
-  ; proto_message_decidable := icomposed_proto_message_decidable IS
-  ; initial_state_prop := icomposed_initial_state_prop IS
-  ; protocol_state_inhabited := icomposed_protocol_state_inhabited IS
-  ; initial_message_prop := icomposed_initial_message_prop IS
-  ; message_inhabited := icomposed_message_inhabited IS Hi
-  ; label_inhabited := icomposed_label_inhabited IS Hi
-  ; transition := icomposed_transition IS
-  ; valid := icomposed_valid_constrained IS constraint
-  ; valid_decidable := icomposed_valid_constrained_decidable IS constraint_decidable
-  |}.
-
-Class composed_vlsm_class (message : Type) `{VLSM message} :=
-  { index : Set
-  ; iproto_state : index -> Type
-  ; istate_proj : forall i : index, state -> iproto_state i
-  ; ilabel : label -> index
-  }.
-
-Definition istate
-  { message : Type }
-  `{composed_vlsm_class message}
-  (i : index)
-  :=
-  { is : iproto_state i | exists s : state, istate_proj i s = is }.
-
-Definition proj_istate
-  { message : Type }
-  `{composed_vlsm_class message}
-  (s : state)
-  (i : index)
-  : istate i.
-remember (istate_proj i s) as is.
-assert (His : exists s', istate_proj i s' = is) by (exists s; subst; reflexivity).
-exact (exist _ is His).
-Defined.
-
-Definition composed_vlsm_istate
-  {oindex : Set} {message : Type} `{Heqd : EqDec oindex}
-  {IS : oindex -> VLSM message}
-  {Hi : inhabited oindex}
-  (i : oindex)
-  : Type
-  := @state message (IS i).
-
-Definition composed_vlsm_istate_proj
-  {oindex : Set} {message : Type} `{Heqd : EqDec oindex}
-  {IS : oindex -> VLSM message}
-  {Hi : inhabited oindex}
-  (i : oindex)
-  (s : @state _ (composed_vlsm IS Hi))
-  : @composed_vlsm_istate oindex message Heqd IS Hi i
-  :=
-  s i.
-
-Definition composed_vlsm_ilabel
-  {oindex : Set} {message : Type} `{Heqd : EqDec oindex}
-  {IS : oindex -> VLSM message}
-  {Hi : inhabited oindex}
-  (l : @label message (composed_vlsm IS Hi))
-  : oindex
-  :=
-  projT1 l.
-
-Definition composed_vlsm_class_instance
-  {oindex : Set} {message : Type} `{Heqd : EqDec oindex}
-  {IS : oindex -> VLSM message}
-  {Hi : inhabited oindex}
-  : @composed_vlsm_class message (composed_vlsm IS Hi) :=
-  {| index := oindex
-  ; iproto_state := @composed_vlsm_istate oindex message Heqd IS Hi
-  ; istate_proj := @composed_vlsm_istate_proj oindex message Heqd IS Hi
-  ; ilabel := composed_vlsm_ilabel
-  |}.
-
-
-
-Definition composed_vlsm_constrained_istate_proj
-  {oindex : Set} {message : Type} `{Heqd : EqDec oindex}
-  {IS : oindex -> VLSM message}
-  {Hi : inhabited oindex}
-  (constraint : icomposed_label IS -> icomposed_state IS * option (icomposed_proto_message IS) -> Prop)
-  (constraint_decidable : forall (l : icomposed_label IS) (som : icomposed_state IS * option (icomposed_proto_message IS)), {constraint l som} + {~constraint l som})
-  (i : oindex)
-  (s : @state _ (composed_vlsm_constrained IS Hi constraint constraint_decidable))
-  : @composed_vlsm_istate oindex message Heqd IS Hi i
-  :=
-  s i.
-
-Definition composed_vlsm_constrained_ilabel
-  {oindex : Set} {message : Type} `{Heqd : EqDec oindex}
-  {IS : oindex -> VLSM message}
-  {Hi : inhabited oindex}
-  (constraint : icomposed_label IS -> icomposed_state IS * option (icomposed_proto_message IS) -> Prop)
-  (constraint_decidable : forall (l : icomposed_label IS) (som : icomposed_state IS * option (icomposed_proto_message IS)), {constraint l som} + {~constraint l som})
-  (l : @label message (composed_vlsm_constrained IS Hi constraint constraint_decidable))
-  : oindex
-  :=
-  projT1 l.
-
-
-Definition composed_vlsm_constrained_instance
-  {oindex : Set} {message : Type} `{Heqd : EqDec oindex}
-  (IS : oindex -> VLSM message)
-  (Hi : inhabited oindex)
-  (constraint : icomposed_label IS -> icomposed_state IS * option (icomposed_proto_message IS) -> Prop)
-  (constraint_decidable : forall (l : icomposed_label IS) (som : icomposed_state IS * option (icomposed_proto_message IS)), {constraint l som} + {~constraint l som})
-  : @composed_vlsm_class message (composed_vlsm_constrained IS Hi constraint constraint_decidable) :=
-  {| index := oindex
-  ; iproto_state := @composed_vlsm_istate oindex message Heqd IS Hi
-  ; istate_proj := @composed_vlsm_constrained_istate_proj oindex message Heqd IS Hi constraint constraint_decidable
-  ; ilabel := composed_vlsm_constrained_ilabel constraint constraint_decidable
+  {| state := indexed_state IS
+  ; label := indexed_label IS
+  ; proto_message_prop := indexed_proto_message_prop IS
+  ; proto_message_decidable := indexed_proto_message_decidable IS
+  ; initial_state_prop := indexed_initial_state_prop IS
+  ; protocol_state_inhabited := indexed_protocol_state_inhabited IS
+  ; initial_message_prop := indexed_initial_message_prop IS
+  ; message_inhabited := indexed_message_inhabited IS Hi
+  ; label_inhabited := indexed_label_inhabited IS Hi
+  ; transition := indexed_transition IS
+  ; valid := indexed_valid_constrained IS constraint
+  ; valid_decidable := indexed_valid_constrained_decidable IS constraint_decidable
   |}.
